{
 "cells": [
  {
   "cell_type": "markdown",
   "id": "2e0a598f",
   "metadata": {},
   "source": [
    "## Written Assignment"
   ]
  },
  {
   "cell_type": "markdown",
   "id": "80278c15",
   "metadata": {},
   "source": [
    "### Problem 1\n",
    "Given \n",
    "$$\n",
    "f(x) = \\frac{1}{\\sqrt{(2\\pi)^k |\\Sigma|}}\n",
    "\\exp\\!\\left(-\\frac{1}{2}(x-\\mu)^T \\Sigma^{-1} (x-\\mu)\\right),\n",
    "$$  \n",
    "\n",
    "where $x, \\mu \\in \\mathbb{R}^k$, and $\\Sigma$ is a $k\\times k$ positive definite matrix with determinant $|\\Sigma|$.  \n",
    "Show that $\\int_{\\mathbb{R}^k} f(x)\\,dx = 1.$  \n",
    "\n",
    "---\n",
    "*對角化 \\\n",
    "$\\Sigma$ can be diagonalized as  \n",
    "\n",
    "$$\n",
    "\\Sigma = Q D Q^T,\n",
    "$$  \n",
    "\n",
    "where $Q$ is an orthogonal matrix and $D$ is diagonal martix. \\\n",
    "Then, $\\Sigma^{1/2} = Q D^{1/2} Q^T$  \n",
    "\n",
    "so $\\Sigma = \\Sigma^{1/2}\\Sigma^{1/2} $ and $\\det(\\Sigma^{1/2}) = \\sqrt{|\\Sigma|}$.  \n",
    "\n",
    "*變數變換 \\\n",
    "Change the variable \n",
    "$$\n",
    "y = \\Sigma^{-1/2}(x - \\mu)\n",
    "\\quad \\Longrightarrow \\quad\n",
    "x = \\mu + \\Sigma^{1/2} y.\n",
    "$$  \n",
    "\n",
    "And Jacobian determinant is $|\\det(\\Sigma^{1/2})| = |\\Sigma|^{1/2}$,  \n",
    "so $dx = |\\Sigma|^{1/2}\\, dy$.  \n",
    "\n",
    "Then,\n",
    "\n",
    "\n",
    "$$\n",
    "\\begin{aligned}\n",
    "\\int_{\\mathbb{R}^k} f(x)\\,dx\n",
    "&= \\frac{1}{\\sqrt{(2\\pi)^k |\\Sigma|}}\n",
    "   \\int_{\\mathbb{R}^k}\n",
    "   \\exp\\!\\left(-\\frac{1}{2}(x-\\mu)^T \\Sigma^{-1} (x-\\mu)\\right)\\,dx \\\\[6pt]\n",
    "&= \\frac{1}{\\sqrt{(2\\pi)^k |\\Sigma|}}\n",
    "   \\int_{\\mathbb{R}^k}\n",
    "   \\exp\\!\\left(-\\frac{1}{2} y^T y\\right)\n",
    "   |\\Sigma|^{1/2}\\,dy \\\\[6pt]\n",
    "&= \\frac{1}{(\\sqrt{2\\pi})^{k}}\n",
    "   \\int_{\\mathbb{R}^k} e^{-\\frac{1}{2}\\sum_{i=1}^k y_i^2}\\,dy \\\\[6pt]\n",
    "&= \\frac{1}{(\\sqrt{2\\pi})^{k}}\n",
    "   \\prod_{i=1}^k \\int_{-\\infty}^{\\infty} e^{-y_i^2/2}\\,dy_i \\\\[6pt]\n",
    "&= \\frac{1}{(\\sqrt{2\\pi})^{k}}\n",
    "   \\left(\\int_{-\\infty}^{\\infty} e^{-y^2/2}\\,dy\\right)^k \\\\[6pt]\n",
    "&= \\frac{1}{(\\sqrt{2\\pi})^{k}}\n",
    "   \\left(\\sqrt{2\\pi}\\right)^k \\\\[6pt]\n",
    "&= 1\n",
    "\\end{aligned}\n",
    "$$\n",
    "** By Calculus ** \n",
    "\n",
    "$\\int_{-\\infty}^{\\infty} e^{-y^2/2}\\,dy = \\sqrt{2\\pi},$\n",
    "\n",
    "Thus, \n",
    "$$\n",
    "\\boxed{\\displaystyle \\int_{\\mathbb{R}^k} f(x)\\,dx = 1.}\n",
    "$$\n",
    "\n",
    "---"
   ]
  },
  {
   "cell_type": "markdown",
   "id": "cb4f6810",
   "metadata": {},
   "source": [
    "### Problem 2\n",
    "Let $A,B$ be $n$-by-$n$ matrices and $x$ be a $n$-by-1 vector.\n",
    "\n",
    "#### (1)Show that $\\frac{\\partial}{\\partial A} \\text{trace}(AB) = B^T$\n",
    "\n",
    "We know\n",
    "$$\n",
    "\\text{tr}(AB) = \\sum_{i=1}^{n} \\sum_{k=1}^{n} a_{ik}b_{ki}\n",
    "$$\n",
    "\n",
    "The derivative is：\n",
    "\n",
    "$$\n",
    "\\frac{\\partial}{\\partial A_{lm}} \\sum_k A_{ik} B_{ki} \n",
    "= \\sum_k \\frac{\\partial A_{ik}}{\\partial A_{lm}} B_{ki}.\n",
    "= \\sum_k \\delta_{il} \\delta_{km} B_{ki}\n",
    "= \\delta_{il} \\sum_k \\delta_{km} B_{ki} = \\delta_{il} B_{mi}\n",
    "$$\n",
    "\n",
    "Thus, \n",
    "$$\n",
    "\\frac{\\partial}{\\partial A_{lm}} \\operatorname{trace}(AB) \n",
    "= \\sum_i \\delta_{il} B_{mi} = B_{ml} = B^T.\n",
    "$$\n",
    "\n",
    "---"
   ]
  },
  {
   "cell_type": "markdown",
   "id": "532a1911",
   "metadata": {},
   "source": [
    "#### (2)Show that $x^TAx=\\text{trace} (xx^TA)$\n",
    "Left:\n",
    "$$\n",
    "\\mathbf{x}^{\\mathsf{T}}\\mathbf{Ax} = \\sum_{i=1}^{n} x_i (\\mathbf{Ax})_i\n",
    "= \\sum_{i=1}^{n} x_i \\left( \\sum_{j=1}^{n} A_{ij} x_j \\right) = \\sum_{i=1}^{n} \\sum_{j=1}^{n} x_i A_{ij} x_j\n",
    "$$\n",
    "\n",
    "\n",
    "Right:\n",
    "$$\n",
    "\\text{trace}(\\mathbf{xx}^{\\mathsf{T}}\\mathbf{A}) \n",
    "= \\sum_{k=1}^{n} (\\mathbf{xx}^{\\mathsf{T}}\\mathbf{A})_{kk}\n",
    "=  \\sum_{k=1}^{n} \\sum_{j=1}^{n} (\\mathbf{xx}^{\\mathsf{T}})_{kj} A_{jk}\n",
    "= \\sum_{k=1}^{n} \\left( \\sum_{j=1}^{n} x_k x_j A_{jk} \\right) = \\sum_{k=1}^{n} \\sum_{j=1}^{n} x_k A_{jk} x_j\n",
    "$$\n",
    "\n",
    "Thus, $x^TAx=\\text{trace} (xx^TA)$\n",
    "\n",
    "---"
   ]
  },
  {
   "cell_type": "markdown",
   "id": "8be634b3",
   "metadata": {},
   "source": [
    "#### (3)Derive the maximum likelihood estimators for a multivariate Gaussian.\n",
    "\n",
    "we have\n",
    "\n",
    "$$\n",
    "\\ell(\\mu, \\Sigma)\n",
    "= -\\frac{N k}{2}\\ln(2\\pi)\n",
    "-\\frac{N}{2}\\ln|\\Sigma|\n",
    "-\\frac{1}{2}\\sum_{i=1}^N (x_i - \\mu)^T \\Sigma^{-1} (x_i - \\mu)\n",
    "$$\n",
    "---"
   ]
  },
  {
   "cell_type": "markdown",
   "id": "da719cc9",
   "metadata": {},
   "source": [
    "\n",
    "\n",
    "\n",
    "$$\n",
    "\\textbf{MLE of } \\mu\n",
    "$$\n",
    "\n",
    "$$\n",
    "\\ell(\\mu) = -\\frac{1}{2}\\sum_{i=1}^N (x_i-\\mu)^T\\Sigma^{-1}(x_i-\\mu) + \\text{const}.\n",
    "$$\n",
    "\n",
    "Then, \n",
    "$$\n",
    "\\frac{\\partial\\ell}{\\partial\\mu}\n",
    "= -\\frac{1}{2}\\frac{\\partial}{\\partial\\mu}\\left[\\sum_{i=1}^N (x_i-\\mu)^T\\Sigma^{-1}(x_i-\\mu)\\right]\n",
    "=-\\frac{1}{2}\\frac{\\partial}{\\partial\\mu}\\left[\\sum_{i=1}^N  x_i^T {\\Sigma}^{-1} x_i - 2x_i^T \\Sigma^{-1} {\\mu} + \\mu^T \\Sigma^{-1} \\mu  \\right]\n",
    "= \\Sigma^{-1}\\sum_{i=1}^N (x_i-\\mu).\n",
    "$$\n",
    "\n",
    "Let $\\frac{\\partial\\ell}{\\partial\\mu}=0$,\n",
    "$$\n",
    "\\Sigma^{-1}\\sum_{i=1}^N (x_i-\\mu)=0 \\quad\\Longrightarrow\\quad \\sum_{i=1}^N (x_i-\\mu)=0.\n",
    "$$\n",
    "\n",
    "Thus, \n",
    "$$\n",
    "\\boxed{\\ \\hat{\\mu}_{\\mathrm{MLE}}=\\frac{1}{N}\\sum_{i=1}^N x_i\\ }.\n",
    "$$\n",
    "\n",
    "---\n",
    "\n"
   ]
  },
  {
   "cell_type": "markdown",
   "id": "e93bca18",
   "metadata": {},
   "source": [
    "$$\n",
    "\\textbf{MLE of } \\Sigma\n",
    "$$\n",
    "\n",
    "\n",
    "$$\n",
    "\\ell(\\Sigma)\n",
    "= -\\frac{N}{2}\\ln|\\Sigma|\n",
    "-\\frac{1}{2}\\sum_{i=1}^N (x_i-\\mu)^T\\Sigma^{-1}(x_i-\\mu)\n",
    "+ \\text{const}.\n",
    "$$\n",
    "\n",
    "$$\n",
    "\\frac{\\partial \\ell}{\\partial\\Sigma}\n",
    "= -\\frac{N}{2} \\frac{\\partial ln|\\Sigma|}{\\partial\\Sigma}\n",
    "-\\frac{1}{2}\\sum_{i=1}^N \\frac{\\partial}{\\partial\\Sigma}(x_i-\\mu)^T\\Sigma^{-1}(x_i-\\mu)\n",
    "$$\n",
    "\n",
    "\n",
    "Solve 1. $\\frac{\\partial ln|\\Sigma|}{\\partial\\Sigma}$\n",
    "\n",
    "We have\n",
    "\n",
    "$d(ln|\\Sigma|) = \\frac{1}{|\\Sigma|} d|\\Sigma| = tr(\\Sigma^{-1} d\\Sigma)$\n",
    "\n",
    "Thus, \n",
    "$\\frac{\\partial ln|\\Sigma|}{\\partial\\Sigma}=(\\Sigma^{-1})^T=\\Sigma^{-1}$\n",
    "\n",
    "Solve 2.$\\frac{\\partial}{\\partial\\Sigma}(x_i-\\mu)^T\\Sigma^{-1}(x_i-\\mu)$\n",
    "\n",
    "Because $(x_i-\\mu)^T\\Sigma^{-1}(x_i-\\mu) = tr((x_i-\\mu)(x_i-\\mu)^T\\Sigma^{-1}) = (x_i-\\mu)(x_i-\\mu)^T$\n",
    "\n",
    "And proposition $\\frac{\\partial}{\\partial A} f(A^{-1}) = -A^T(\\frac {\\partial}{\\partial A^{-1}}f(A^{-1}))A^{-T}$\n",
    "\n",
    "Then, $\\frac{\\partial}{\\partial\\Sigma}(x_i-\\mu)^T\\Sigma^{-1}(x_i-\\mu) = -\\Sigma^{-1}(x_i-\\mu)(x_i-\\mu)^T\\Sigma^{-1}$\n",
    "\n",
    "So,\n",
    "$$\n",
    "\\frac{\\partial \\ell}{\\partial\\Sigma}\n",
    "= -\\frac{N}{2} \\Sigma^{-1}\n",
    "+\\frac{1}{2}\\sum_{i=1}^N \\Sigma^{-1}(x_i-\\mu)(x_i-\\mu)^T\\Sigma^{-1}\n",
    "$$\n",
    "\n",
    "\n",
    "Let $\\frac{\\partial \\ell}{\\partial\\Sigma} = 0$\n",
    "\n",
    "\n",
    "$$\n",
    "\\sum_{i=1}^N (x_i-\\hat\\mu)(x_i-\\hat\\mu)^T = N\\Sigma.\n",
    "$$\n",
    "\n",
    "Thus,\n",
    "\n",
    "$$\n",
    "\\boxed{\\ \\widehat{\\Sigma}_{\\mathrm{MLE}}\n",
    "= \\frac{1}{N}\\sum_{i=1}^N (x_i-\\hat\\mu)(x_i-\\hat\\mu)^T\\ }.\n",
    "$$\n",
    "\n",
    "---\n"
   ]
  },
  {
   "cell_type": "markdown",
   "id": "86ef1bc4",
   "metadata": {},
   "source": [
    "### Problem 3 - unanswer question\n",
    "\n",
    "\n",
    "#### What may happened when the if the real-world data we used doesn't satisfied normal distribution? What is the result?"
   ]
  }
 ],
 "metadata": {
  "language_info": {
   "name": "python"
  }
 },
 "nbformat": 4,
 "nbformat_minor": 5
}
